split rule annotation and elaboration

_build/default/theories/CaseStudies/MiniML/driver/.McptsLib.objs/mcptsLib__Test.impl.d
@@ -1,1 +1,1 @@
-theories/CaseStudies/MiniML/driver/Test.pp.ml: Expect_test_collector Expect_test_common Expect_test_config Inline_test_config Main McptsExtracted Ppx_inline_test_lib
+theories/CaseStudies/MiniML/driver/Test.pp.ml: Expect_test_config Inline_test_config Main McptsExtracted Ppx_expect_runtime Ppx_inline_test_lib
