_build/default/theories/CaseStudies/MiniML/driver/extracted/.McptsExtracted.objs/mcptsExtracted__Frontend.impl.d
@@ -1,1 +1,1 @@
-theories/CaseStudies/MiniML/driver/extracted/Frontend.ml: Nat Obj Signature Stdlib Syntax
+theories/CaseStudies/MiniML/driver/extracted/Frontend.ml: CstAnn Elaborator Obj Signature Syntax
