_build/default/theories/CaseStudies/MiniML/driver/extracted/Frontend.ml
@@ -1,19 +1,8 @@
-open Nat
+open Elaborator
 open Signature
 open Syntax
 
 let __ = let rec f _ = Obj.repr f in Obj.repr f
-
-(** val lookup : string -> string list -> int option **)
-
-let rec lookup s = function
-| [] -> None
-| c :: cs ->
-  if (=) c s
-  then Some 0
-  else (match lookup s cs with
-        | Some n -> Some (add n (Stdlib.Int.succ 0))
-        | None -> None)
 
 module Cst =
  struct
@@ -29,59 +18,27 @@ module Cst =
   | Coq_natrec of obj * string * obj * obj * string * string * obj
  end
 
+(** val annotate' : Cst.obj -> CstAnn.obj **)
+
+let rec annotate' = function
+| Cst.Coq_st -> CstAnn.Coq_st (Obj.magic Coq_s_typ)
+| Cst.Coq_pi (s, t, c) ->
+  CstAnn.Coq_pi ((Obj.magic Coq_s_typ), (Obj.magic Coq_s_typ),
+    (Obj.magic Coq_s_typ), (Obj.magic __), s, (annotate' t), (annotate' c))
+| Cst.Coq_fn (s, t, b, c) ->
+  CstAnn.Coq_fn ((Obj.magic Coq_s_typ), (Obj.magic Coq_s_typ),
+    (Obj.magic Coq_s_typ), (Obj.magic __), s, (annotate' t), (annotate' b),
+    (annotate' c))
+| Cst.Coq_app (c1, c2) -> CstAnn.Coq_app ((annotate' c1), (annotate' c2))
+| Cst.Coq_var x -> CstAnn.Coq_var x
+| Cst.Coq_nat -> CstAnn.Coq_nat
+| Cst.Coq_zero -> CstAnn.Coq_zero
+| Cst.Coq_succ c -> CstAnn.Coq_succ (annotate' c)
+| Cst.Coq_natrec (n, mx, m, z, sx, sr, s) ->
+  CstAnn.Coq_natrec ((annotate' n), mx, (annotate' m), (annotate' z), sx, sr,
+    (annotate' s))
+
 (** val elaborate' : Cst.obj -> string list -> exp option **)
 
-let rec elaborate' cst ctx =
-  match cst with
-  | Cst.Coq_st -> Some (Coq_a_st (Obj.magic Coq_s_typ))
-  | Cst.Coq_pi (s, t, c) ->
-    (match elaborate' c (s :: ctx) with
-     | Some a ->
-       (match elaborate' t ctx with
-        | Some t0 ->
-          Some (Coq_a_pi ((Obj.magic Coq_s_typ), (Obj.magic Coq_s_typ),
-            (Obj.magic Coq_s_typ), (Obj.magic __), t0, a))
-        | None -> None)
-     | None -> None)
-  | Cst.Coq_fn (s, t, b, c) ->
-    (match elaborate' c (s :: ctx) with
-     | Some a ->
-       (match elaborate' b (s :: ctx) with
-        | Some b0 ->
-          (match elaborate' t ctx with
-           | Some t0 ->
-             Some (Coq_a_fn ((Obj.magic Coq_s_typ), (Obj.magic Coq_s_typ),
-               (Obj.magic Coq_s_typ), (Obj.magic __), t0, b0, a))
-           | None -> None)
-        | None -> None)
-     | None -> None)
-  | Cst.Coq_app (c1, c2) ->
-    (match elaborate' c1 ctx with
-     | Some a1 ->
-       (match elaborate' c2 ctx with
-        | Some a2 -> Some (Coq_a_app (a1, a2))
-        | None -> None)
-     | None -> None)
-  | Cst.Coq_var x ->
-    (match lookup x ctx with
-     | Some n -> Some (Coq_a_var n)
-     | None -> None)
-  | Cst.Coq_nat -> Some Coq_a_nat
-  | Cst.Coq_zero -> Some Coq_a_zero
-  | Cst.Coq_succ c ->
-    (match elaborate' c ctx with
-     | Some a -> Some (Coq_a_succ a)
-     | None -> None)
-  | Cst.Coq_natrec (n, mx, m, z, sx, sr, s) ->
-    (match elaborate' m (mx :: ctx) with
-     | Some m0 ->
-       (match elaborate' z ctx with
-        | Some z0 ->
-          (match elaborate' s (sr :: (sx :: ctx)) with
-           | Some s0 ->
-             (match elaborate' n ctx with
-              | Some n0 -> Some (Coq_a_natrec (m0, z0, s0, n0))
-              | None -> None)
-           | None -> None)
-        | None -> None)
-     | None -> None)
+let elaborate' cst ctx =
+  elaborate coq_MiniML_Sig (annotate' cst) ctx
